Lambda/PCF/Adequacy.lean
@@ -1,0 +1,232 @@
+import Lambda.PCF.Denotational
+
+namespace PCF
+
+def R : (T : Ty) → Term ∅ T → ⟦T⟧ᵀ → Prop
+| TBool, t, d =>
+  (d = some true → t ⟶* Term.true) ∧
+  (d = some false → t ⟶* Term.false)
+| TNat, t, d =>
+  ∀ n, d = some n → t ⟶* Term.nat n
+| T₁ ⇒ T₂, t, d =>
+  ∀ t' d', R T₁ t' d' → R T₂ (t ⬝ t') (d d')
+| T₁ * T₂, t, ⟨d₁, d₂⟩ =>
+  R T₁ (Term.fst t) d₁ ∧ R T₂ (Term.snd t) d₂
+
+lemma R.bot : R T t ⊥ := by
+  induction T with
+  | bool => constructor <;> intro <;> contradiction
+  | nat => intro _ _; contradiction
+  | fn T₁ T₂ _ ih₂ =>
+    intro t' d' _; exact ih₂
+  | prod T₁ T₂ ih₁ ih₂ =>
+    exact ⟨ih₁, ih₂⟩
+
+theorem R.le {d d' : ⟦T⟧ᵀ} :
+  d' ≤ d → R T t d → R T t d' := by
+  intro h₁ h₂
+  induction T with
+  | bool =>
+    cases' d with b <;> cases' d' with b' <;>
+      cases h₁ <;> try assumption
+    exact bot
+  | nat =>
+    cases' d with n <;> cases' d' with n' <;>
+      cases h₁ <;> try assumption
+    exact bot
+  | fn T₁ T₂ _ ih₂ =>
+    intro t' d₁ h₃
+    apply ih₂
+    · apply h₁
+    · apply h₂; exact h₃
+  | prod T₁ T₂ ih₁ ih₂ =>
+    cases' d with d₁ d₂
+    cases' d' with d₁' d₂'
+    cases' h₁ with h₁ h₁'
+    constructor
+    · exact ih₁ h₁ h₂.left
+    · exact ih₂ h₁' h₂.right
+
+theorem R.sup {s : Set ⟦T⟧ᵀ} {hs : Directed' s} :
+  (∀ x ∈ s, R T t x) → R T t (Dcpo.sSup s hs) := by
+  intro h
+  induction T with
+  | bool | nat =>
+    rcases Domain.Flat.directed_cases hs with h₁ | ⟨x, h₁⟩ | ⟨x, h₁⟩ <;>
+      subst h₁ <;> simp [Dcpo.sSup_singleton, Dcpo.sSup_pair bot_le] <;>
+      apply h <;> aesop
+  | fn T₁ T₂ _ ih₂ =>
+    intro t' d h₁
+    apply ih₂
+    intro _ ⟨f, h₂, h₃⟩
+    subst h₃
+    apply h _ h₂
+    exact h₁
+  | prod T₁ T₂ ih₁ ih₂ =>
+    constructor
+    · apply ih₁
+      intro _ ⟨⟨d₁, d₂⟩, h₁, h₂⟩; subst h₂
+      exact (h _ h₁).left
+    · apply ih₂
+      intro _ ⟨⟨d₁, d₂⟩, h₁, h₂⟩; subst h₂
+      exact (h _ h₁).right
+
+theorem R.inv_step {t t' : Term ∅ T} :
+  t ⟶ t' → R T t' d → R T t d := by
+  intro h₁ h₂
+  induction T with
+  | bool =>
+    constructor <;> intro h₃ <;> apply Rel.Multi.step h₁
+    · exact h₂.left h₃
+    · exact h₂.right h₃
+  | nat =>
+    intro _ h₃; apply Rel.Multi.step h₁; exact h₂ _ h₃
+  | fn T₁ T₂ _ ih₂ =>
+    intro t' d' h₃
+    apply ih₂ (Step.app₁ h₁)
+    apply h₂
+    · exact h₃
+  | prod T₁ T₂ ih₁ ih₂ =>
+    constructor
+    · exact ih₁ (Step.fst h₁) h₂.left
+    · exact ih₂ (Step.snd h₁) h₂.right
+
+theorem R.inv_reduce {t t' : Term ∅ T} :
+  t ⟶* t' → R T t' d → R T t d := by
+  intro h₁ h₂
+  induction h₁ with
+  | refl => exact h₂
+  | step h₁ _ ih => apply inv_step h₁; exact ih h₂
+
+def Rsub (σ : Subst Γ ∅) (g : ⟦Γ⟧ᴳ) :=
+  ∀ T (x : T ∈' Γ), R T (σ x) (Con.denot_get x g)
+
+theorem R.fundamental :
+  Rsub σ g → R T (t[σ]ˢ) (⟦t⟧ᵗ g) := by
+  intro h
+  induction t with simp [Term.denot]
+  | var x => apply h
+  | lam t ih =>
+    intro t' d h₁'
+    apply inv_step Step.beta
+    simp [Term.subst_comp]
+    apply ih
+    intro _ x
+    cases x with
+    | fz => exact h₁'
+    | fs x =>
+      simp [Subst.comp, Subst.lift, Term.shift_subst_single, Con.denot_get]
+      apply h
+  | app t₁ t₂ ih₁ ih₂ =>
+    apply ih₁ h
+    exact ih₂ h
+  | fix t ih =>
+    apply sup
+    intro _ ⟨n, h₁⟩; subst h₁
+    induction' n with n ih'
+    · exact bot
+    · simp [Domain.iter]
+      apply inv_step Step.fix₂
+      apply ih h
+      exact ih'
+  | true | false =>
+    constructor <;> intro h <;> cases h; constructor
+  | ite t₁ t₂ t₃ ih₁ ih₂ ih₃ =>
+    simp [Domain.ite]; split
+    next h₁ =>
+      apply (ih₁ h).left at h₁
+      apply inv_reduce
+      · apply Rel.Multi.congr h₁ Step.ite₁
+      · apply inv_step Step.ite_true
+        exact ih₂ h
+    next h₁ =>
+      apply (ih₁ h).right at h₁
+      apply inv_reduce
+      · apply Rel.Multi.congr h₁ Step.ite₁
+      · apply inv_step Step.ite_false
+        exact ih₃ h
+    next => exact bot
+  | nat n => intro _ h; cases h; constructor
+  | succ t ih =>
+    simp [Domain.succ]; split
+    next h₁ =>
+      apply ih h at h₁
+      apply inv_reduce
+      · apply Rel.Multi.congr h₁ Step.succ
+      · apply inv_step Step.succ_nat
+        intro _ h; cases h; constructor
+    next => exact bot
+  | pred t ih =>
+    simp [Domain.pred]; split
+    next h₁ =>
+      apply ih h at h₁
+      apply inv_reduce
+      · apply Rel.Multi.congr h₁ Step.pred
+      · apply inv_step Step.pred_zero
+        intro _ h; cases h; constructor
+    next h₁ =>
+      apply ih h at h₁
+      apply inv_reduce
+      · apply Rel.Multi.congr h₁ Step.pred
+      · apply inv_step Step.pred_succ
+        intro _ h; cases h; constructor
+    next => exact bot
+  | isz t ih =>
+    simp [Domain.isz]; split
+    next h₁ =>
+      apply ih h at h₁
+      apply inv_reduce
+      · apply Rel.Multi.congr h₁ Step.isz
+      · apply inv_step Step.isz_zero
+        constructor <;> intro h <;> cases h; constructor
+    next h₁ =>
+      apply ih h at h₁
+      apply inv_reduce
+      · apply Rel.Multi.congr h₁ Step.isz
+      · apply inv_step Step.isz_succ
+        constructor <;> intro h <;> cases h; constructor
+    next => exact bot
+  | pair t₁ t₂ ih₁ ih₂ =>
+    constructor
+    · apply inv_step Step.sigma₁; exact ih₁ h
+    · apply inv_step Step.sigma₂; exact ih₂ h
+  | fst t ih => exact (ih h).left
+  | snd t ih => exact (ih h).right
+
+
+
+theorem adequacy {v t : Term ∅ T} :
+  Value v → ⟦t⟧ᵗ () = ⟦v⟧ᵗ () → t ⟶* v := by
+  intro h₁ h₂
+  have h₃ : R T t (⟦t⟧ᵗ ()) := by
+    conv => arg 2; rw [←Term.subst_id (t := t)]
+    apply R.fundamental
+    intro _ x; cases x
+  rw [h₂] at h₃
+  cases v with simp [Value] at h₁
+  | true => exact h₃.left rfl
+  | false => exact h₃.right rfl
+  | nat n => exact h₃ n rfl
+
+lemma denot_value_le {v : Term ∅ T} :
+  Value v → ⟦v⟧ᵗ () ≤ d → d = ⟦v⟧ᵗ () := by
+  intro h₁ h₂
+  cases v <;> simp [Value, Term.denot] at * <;>
+    cases d <;> cases h₂ <;> rfl
+
+theorem denot_le_implies_context_approx :
+  ⟦t₁⟧ᵗ ≤ ⟦t₂⟧ᵗ → t₁ ≲ᶜ t₂ := by
+  intro h₁ T C v h₂ h₃
+  apply Reduce.denot_eq at h₃
+  apply adequacy h₂
+  apply denot_value_le h₂
+  simp [←h₃, Context.denot_plug]
+  apply ⟦C⟧ᶜ.2.mono
+  exact h₁
+
+theorem denot_eq_implies_context_equiv :
+  ⟦t₁⟧ᵗ = ⟦t₂⟧ᵗ → t₁ ≈ᶜ t₂ := by
+  intro h₁ T C v h₂
+  constructor <;> apply denot_le_implies_context_approx <;> aesop
+
+end PCF
