Lambda/PCF/Denotational.lean
@@ -1,0 +1,222 @@
+import Lambda.PCF.Operational
+import Lambda.Domain
+
+noncomputable section
+
+namespace Domain
+
+variable {α : Domain}
+
+def Bool' := Flat Bool
+
+def ite : Bool' →ᴰ α →ᴰ α →ᴰ α where
+  val := λ
+         | some true => K
+         | some false => swap K
+         | none => ⊥
+  property := by
+    apply Flat.mono_continuous
+    intro b₁ b₂ h; simp
+    split <;> split <;> cases h <;> simp
+
+def Nat' := Flat Nat
+
+def succ : Nat' →ᴰ Nat' where
+  val := λ
+         | some n => some (n + 1)
+         | none => ⊥
+  property := by
+    apply Flat.mono_continuous
+    intros x₁ x₂ h; simp
+    split <;> split <;> cases h <;> simp
+
+def pred : Nat' →ᴰ Nat' where
+  val := λ
+         | some 0 => some 0
+         | some (n + 1) => some n
+         | none => ⊥
+  property := by
+    apply Flat.mono_continuous
+    intros x₁ x₂ h; simp
+    split <;> split <;> cases h <;> constructor
+
+def isz : Nat' →ᴰ Bool' where
+  val := λ
+         | some 0 => some true
+         | some (_ + 1) => some false
+         | none => ⊥
+  property := by
+    apply Flat.mono_continuous
+    intros x₁ x₂ h; simp
+    split <;> split <;> cases h <;> constructor
+
+end Domain
+
+namespace PCF
+
+@[reducible] def Ty.Denot : Ty → Domain
+| bool => Domain.Bool'
+| nat => Domain.Nat'
+| T₁ * T₂ => T₁.Denot ×ᴰ T₂.Denot
+| fn T₁ T₂ => T₁.Denot →ᴰ T₂.Denot
+notation "⟦" T "⟧ᵀ" => Ty.Denot T
+
+instance : CoeFun (⟦T₁ ⇒ T₂⟧ᵀ) (λ _ => ⟦T₁⟧ᵀ → ⟦T₂⟧ᵀ) := ⟨Subtype.val⟩
+
+def Con.Denot : Con → Domain
+| [] => Domain.Unit
+| Γ,' T => Γ.Denot ×ᴰ ⟦T⟧ᵀ
+notation "⟦" Γ "⟧ᴳ" => Con.Denot Γ
+
+def Con.denot_get : T ∈' Γ → ⟦Γ⟧ᴳ →ᴰ ⟦T⟧ᵀ
+| fz => Domain.snd
+| fs x => Domain.comp (denot_get x) Domain.fst
+
+theorem Con.denot_ext {a b : ⟦Γ⟧ᴳ} :
+  (∀ {T} (x : T ∈' Γ), Con.denot_get x a = Con.denot_get x b) → a = b := by
+  intro h
+  induction' Γ with Γ T ih
+  · rfl
+  · cases' a with a a'; cases' b with b b'
+    congr
+    · apply ih; intros T x
+      replace h := h (x := fs x)
+      simp [denot_get] at h
+      exact h
+    · replace h := h (x := fz)
+      simp [denot_get] at h
+      exact h
+
+def Term.denot : Term Γ T → ⟦Γ⟧ᴳ →ᴰ ⟦T⟧ᵀ
+| #x => Con.denot_get x
+| λ' t => Domain.curry t.denot
+| t₁ ⬝ t₂ => Domain.S t₁.denot t₂.denot
+| fix t => Domain.comp Domain.fix t.denot
+| true => Domain.const (some Bool.true)
+| false => Domain.const (some Bool.false)
+| ite t₁ t₂ t₃ => Domain.comp₃ Domain.ite t₁.denot t₂.denot t₃.denot
+| nat n => Domain.const (some n)
+| succ t => Domain.comp Domain.succ t.denot
+| pred t => Domain.comp Domain.pred t.denot
+| isz t => Domain.comp Domain.isz t.denot
+| ⟪t₁, t₂⟫ => Domain.comp₂ Domain.pair t₁.denot t₂.denot
+| fst t => Domain.comp Domain.fst t.denot
+| snd t => Domain.comp Domain.snd t.denot
+notation "⟦" t "⟧ᵗ" => Term.denot t
+
+def Weaken.denot : Γ ⊆ʷ Δ → ⟦Δ⟧ᴳ →ᴰ ⟦Γ⟧ᴳ
+| εʷ => Domain.I
+| ↑ʷρ => Domain.comp ρ.denot Domain.fst
+| ⇑ʷρ => Domain.uncurry (Domain.comp Domain.pair ρ.denot)
+notation "⟦" ρ "⟧ʷ" => Weaken.denot ρ
+
+lemma Weaken.denot_id : ⟦(idʷ : Γ ⊆ʷ Γ)⟧ʷ = Domain.I := by
+  induction' Γ with Γ T ih
+  · rfl
+  · ext ⟨g, d⟩; simp [Weaken.id, Weaken.denot, ih]
+
+theorem Term.denot_weaken {ρ : Γ ⊆ʷ Δ} :
+  ⟦t[ρ]ʷ⟧ᵗ = Domain.comp ⟦t⟧ᵗ ⟦ρ⟧ʷ := by
+  induction t generalizing Δ <;> simp [Term.weaken, Term.denot]
+  case var x =>
+    induction ρ with
+    | nil => cases x
+    | step ρ ih =>
+      ext ⟨g, d⟩; simp [Weaken.denot, Con.denot_get, ih]
+    | lift ρ ih =>
+      ext ⟨g, d⟩; simp [Weaken.denot]
+      cases x <;> simp [Con.denot_get, ih]
+  all_goals aesop
+
+lemma Term.denot_shift :
+  ⟦(↑ₜt : Term (Γ,' T) T')⟧ᵗ = Domain.comp ⟦t⟧ᵗ Domain.fst := by
+  ext ⟨g, d⟩; simp [Term.shift, Term.denot_weaken, Weaken.denot, Weaken.denot_id]
+
+def Subst.denot (σ : Subst Γ Δ) : ⟦Δ⟧ᴳ →ᴰ ⟦Γ⟧ᴳ :=
+  match Γ with
+  | [] => Domain.const ()
+  | _,' _ => Domain.comp₂ Domain.pair σ.tail.denot σ.head.denot
+notation "⟦" σ "⟧ˢ" => Subst.denot σ
+
+lemma Subst.denot_apply {σ : Subst Γ Δ} {x : T ∈' Γ} :
+  ⟦σ x⟧ᵗ a = Con.denot_get x (⟦σ⟧ˢ a):= by
+  induction' x with _ _ _ x ih <;> simp [Con.denot_get, Subst.denot]
+  · simp [Subst.head]
+  · have h := ih (σ := σ.tail)
+    simp at h; rw [←h]
+    simp [Subst.tail]
+
+theorem Term.denot_subst {t : Term Γ T} {σ : Subst Γ Δ} :
+  ⟦t[σ]ˢ⟧ᵗ = Domain.comp ⟦t⟧ᵗ ⟦σ⟧ˢ := by
+  induction t generalizing Δ <;> simp [Term.subst, Term.denot]
+  case var x => ext g; simp [Subst.denot_apply]
+  case lam t ih =>
+    ext g d
+    simp [ih, Subst.denot]
+    congr!
+    apply Con.denot_ext
+    intros T x
+    simp [←Subst.denot_apply, Subst.tail, Subst.lift, Term.denot_shift]
+  all_goals aesop
+
+theorem Term.denot_subst_single {t₁ : Term (Γ,' T₁) T₂} :
+  ⟦t₁[↦ t₂]ˢ⟧ᵗ = Domain.S (Domain.curry ⟦t₁⟧ᵗ) ⟦t₂⟧ᵗ := by
+  ext g; simp [Term.denot_subst, Subst.denot]
+  congr!
+  simp [Subst.tail, Subst.single]
+  apply Con.denot_ext
+  intros T x
+  simp [←Subst.denot_apply, Term.denot]
+
+def Context.denot : Context Γ T Δ T' → (⟦Γ⟧ᴳ →ᴰ ⟦T⟧ᵀ) →ᴰ (⟦Δ⟧ᴳ →ᴰ ⟦T'⟧ᵀ)
+| hole => Domain.I
+| lam C => Domain.comp Domain.curry C.denot
+| app₁ C t => Domain.comp ((Domain.swap Domain.S) ⟦t⟧ᵗ) C.denot
+| app₂ t C => Domain.comp (Domain.S ⟦t⟧ᵗ) C.denot
+| fix C => Domain.comp (Domain.comp Domain.fix) C.denot
+| ite₁ C t₂ t₃ => Domain.comp (Domain.S (Domain.S (Domain.comp₃ Domain.ite) (Domain.K ⟦t₂⟧ᵗ)) (Domain.K ⟦t₃⟧ᵗ)) C.denot
+| ite₂ t₁ C t₃ => Domain.comp (Domain.S (Domain.comp₃ Domain.ite ⟦t₁⟧ᵗ) (Domain.K ⟦t₃⟧ᵗ)) C.denot
+| ite₃ t₁ t₂ C => Domain.comp (Domain.comp₃ Domain.ite ⟦t₁⟧ᵗ ⟦t₂⟧ᵗ) C.denot
+| succ C => Domain.comp (Domain.comp Domain.succ) C.denot
+| pred C => Domain.comp (Domain.comp Domain.pred) C.denot
+| isz C => Domain.comp (Domain.comp Domain.isz) C.denot
+| pair₁ C t => Domain.comp (Domain.comp₂ (Domain.swap Domain.pair) ⟦t⟧ᵗ) C.denot
+| pair₂ t C => Domain.comp (Domain.comp₂ Domain.pair ⟦t⟧ᵗ) C.denot
+| fst C => Domain.comp (Domain.comp Domain.fst) C.denot
+| snd C => Domain.comp (Domain.comp Domain.snd) C.denot
+notation "⟦" C "⟧ᶜ" => Context.denot C
+
+theorem Context.denot_plug {C : Context Γ T Δ T'} :
+  ⟦C.plug t⟧ᵗ = ⟦C⟧ᶜ ⟦t⟧ᵗ := by
+  induction C <;> ext g <;>
+    simp [Context.plug, Term.denot, Context.denot] <;> aesop
+
+theorem compositionality {C : Context Γ T Δ T'} :
+  ⟦t₁⟧ᵗ = ⟦t₂⟧ᵗ → ⟦C.plug t₁⟧ᵗ = ⟦C.plug t₂⟧ᵗ := by
+  intro h
+  simp [Context.denot_plug, h]
+
+theorem Step.denot_eq : t₁ ⟶ t₂ → ⟦t₁⟧ᵗ = ⟦t₂⟧ᵗ := by
+  intro h
+  induction h <;> ext g <;> simp [Term.denot]
+  case beta =>
+    simp [Term.denot_subst_single]
+  case fix₂ =>
+    simp [Domain.fix_is_fixpoint]
+  all_goals aesop
+
+theorem Reduce.denot_eq : t₁ ⟶* t₂ → ⟦t₁⟧ᵗ = ⟦t₂⟧ᵗ := by
+  intro h; induction h with
+  | refl => rfl
+  | step h _ ih => simp [ih, Step.denot_eq h]
+
+theorem soundness : t₁ ≡ t₂ → ⟦t₁⟧ᵗ = ⟦t₂⟧ᵗ := by
+  intro h; induction h with
+  | refl => rfl
+  | symm _ ih => simp [ih]
+  | trans _ _ ih₁ ih₂ => simp [ih₁, ih₂]
+  | step h => simp [Step.denot_eq h]
+
+end PCF
+
+end
