Lambda/PCF/Syntax.lean
@@ -1,0 +1,298 @@
+import Lambda.Prelude
+import Lambda.Fin
+
+namespace PCF
+
+inductive Ty where
+| bool : Ty
+| nat : Ty
+| fn : Ty → Ty → Ty
+| prod : Ty → Ty → Ty
+infixr:70 (priority := high) " ⇒ " => Ty.fn
+instance : Mul Ty := ⟨Ty.prod⟩
+@[match_pattern] abbrev TBool := Ty.bool
+@[match_pattern] abbrev TNat := Ty.nat
+
+def Con := List Ty
+@[match_pattern] def Con.add (Γ : Con) (T : Ty) := T :: Γ
+instance : EmptyCollection Con := ⟨[]⟩
+infixl:60 ",' " => Con.add
+
+
+
+inductive Term : Con → Ty → Type where
+| var : T ∈' Γ → Term Γ T
+| lam : Term (Γ,' T₁) T₂ → Term Γ (T₁ ⇒ T₂)
+| app : Term Γ (T₁ ⇒ T₂) → Term Γ T₁ → Term Γ T₂
+| fix : Term Γ (T ⇒ T) → Term Γ T
+| true : Term Γ TBool
+| false : Term Γ TBool
+| ite : Term Γ TBool → Term Γ T → Term Γ T → Term Γ T
+| nat : Nat → Term Γ TNat
+| succ : Term Γ TNat → Term Γ TNat
+| pred : Term Γ TNat → Term Γ TNat
+| isz : Term Γ TNat → Term Γ TBool
+| pair : Term Γ T₁ → Term Γ T₂ → Term Γ (T₁ * T₂)
+| fst : Term Γ (T₁ * T₂) → Term Γ T₁
+| snd : Term Γ (T₁ * T₂) → Term Γ T₂
+
+prefix:max "#" => Term.var
+notation "λ'" => Term.lam
+infix:80 " ⬝ " => Term.app
+notation "⟪" t₁ ", " t₂ "⟫" => Term.pair t₁ t₂
+
+
+
+inductive Weaken : Con → Con → Type where
+| nil : Weaken ∅ ∅
+| step : Weaken Γ Δ → Weaken Γ (Δ,' T)
+| lift : Weaken Γ Δ → Weaken (Γ,' T) (Δ,' T)
+infix:50 " ⊆ʷ " => Weaken
+notation "εʷ" => Weaken.nil
+prefix:max "↑ʷ" => Weaken.step
+prefix:max "⇑ʷ" => Weaken.lift
+
+def Weaken.id : Γ ⊆ʷ Γ :=
+  match Γ with
+  | [] => εʷ
+  | _,' _ => ⇑ʷid
+notation "idʷ" => Weaken.id
+
+@[simp] def Weaken.apply : Γ ⊆ʷ Δ → T ∈' Γ → T ∈' Δ
+| ↑ʷρ, x => fs (ρ.apply x)
+| ⇑ʷρ, fz => fz
+| ⇑ʷρ, fs x => fs (ρ.apply x)
+
+@[simp] lemma Weaken.id_apply : idʷ.apply x = x := by
+  rename Con => Γ
+  induction' Γ with Γ T ih <;> simp [Weaken.id]
+  · cases x
+  · cases' x with _ _ _ x
+    · rfl
+    · simp [Weaken.id, ih]
+
+@[simp] def Term.weaken : Term Γ T → Γ ⊆ʷ Δ → Term Δ T
+| #x, ρ => #(ρ.apply x)
+| λ' t, ρ => λ' (t.weaken ⇑ʷρ)
+| t₁ ⬝ t₂, ρ => t₁.weaken ρ ⬝ t₂.weaken ρ
+| fix t, ρ => fix (t.weaken ρ)
+| true, _ => true
+| false, _ => false
+| ite t₁ t₂ t₃, ρ => ite (t₁.weaken ρ) (t₂.weaken ρ) (t₃.weaken ρ)
+| nat n, _ => nat n
+| succ t, ρ => succ (t.weaken ρ)
+| pred t, ρ => pred (t.weaken ρ)
+| isz t, ρ => isz (t.weaken ρ)
+| ⟪t₁, t₂⟫, ρ => ⟪t₁.weaken ρ, t₂.weaken ρ⟫
+| fst t, ρ => fst (t.weaken ρ)
+| snd t, ρ => snd (t.weaken ρ)
+notation t "[" ρ "]ʷ" => Term.weaken t ρ
+
+theorem Term.weaken_id : t[idʷ]ʷ = t := by
+  induction t <;> simp <;> aesop
+
+def Term.shift (t : Term Γ T) : Term (Γ,' T') T := t[↑ʷidʷ]ʷ
+prefix:max "↑ₜ" => Term.shift
+
+def Weaken.comp : Γ ⊆ʷ Δ → Δ ⊆ʷ Θ → Γ ⊆ʷ Θ
+| ρ, εʷ => ρ
+| ρ₁, ↑ʷρ₂ => ↑ʷ(ρ₁.comp ρ₂)
+| ↑ʷρ₁, ⇑ʷρ₂ => ↑ʷ(ρ₁.comp ρ₂)
+| ⇑ʷρ₁, ⇑ʷρ₂ => ⇑ʷ(ρ₁.comp ρ₂)
+infix:70 " ∘ʷ " => Weaken.comp
+
+lemma Weaken.comp_apply {ρ₁ : Γ ⊆ʷ Δ} : (ρ₁ ∘ʷ ρ₂).apply x = ρ₂.apply (ρ₁.apply x) := by
+  induction ρ₂ generalizing Γ <;>
+    cases ρ₁ <;> (try cases x) <;> simp [Weaken.comp] <;> aesop
+
+theorem Term.weaken_comp {ρ₂ : Δ ⊆ʷ Θ} :
+  t[ρ₁]ʷ[ρ₂]ʷ = t[ρ₁ ∘ʷ ρ₂]ʷ := by
+  induction t generalizing Δ Θ ρ₂ <;> simp
+  case var => simp [Weaken.comp_apply]
+  all_goals aesop
+
+
+
+def Subst (Γ Δ : Con) := ∀ ⦃T : Ty⦄, T ∈' Γ → Term Δ T
+
+def Subst.head (σ : Subst (Γ,' T) Δ) : Term Δ T := σ fz
+def Subst.tail (σ : Subst (Γ,' T) Δ) : Subst Γ Δ := λ _ x => σ (fs x)
+
+def Subst.id : Subst Γ Γ := λ _ => Term.var
+notation "idₛ" => Subst.id
+
+def Subst.lift (σ : Subst Γ Δ) : Subst (Γ,' T) (Δ,' T)
+| _, fz => #fz
+| _, fs x => ↑ₜ(σ x)
+prefix:max "⇑" => Subst.lift
+
+def Subst.single (t : Term Γ T) : Subst (Γ,' T) Γ
+| _, fz => t
+| _, fs x => #x
+prefix:max "↦ " => Subst.single
+
+@[simp] def Term.subst : Term Γ T → Subst Γ Δ → Term Δ T
+| #x, σ => σ x
+| λ' t, σ => λ' (t.subst ⇑σ)
+| t₁ ⬝ t₂, σ => t₁.subst σ ⬝ t₂.subst σ
+| fix t, σ => fix (t.subst σ)
+| true, _ => true
+| false, _ => false
+| ite t₁ t₂ t₃, σ => ite (t₁.subst σ) (t₂.subst σ) (t₃.subst σ)
+| nat n, _ => nat n
+| succ t, σ => succ (t.subst σ)
+| pred t, σ => pred (t.subst σ)
+| isz t, σ => isz (t.subst σ)
+| ⟪t₁, t₂⟫, σ => ⟪t₁.subst σ, t₂.subst σ⟫
+| fst t, σ => fst (t.subst σ)
+| snd t, σ => snd (t.subst σ)
+notation t "[" σ "]ˢ" => Term.subst t σ
+
+lemma Term.subst_id {t : Term Γ T} : t[idₛ]ˢ = t := by
+  induction t
+  case lam _ ih =>
+    simp
+    conv => rhs; rw [←ih]
+    congr
+    funext _ x
+    cases x <;> simp [Subst.lift, Subst.id, Term.shift]
+  all_goals aesop
+
+def Weaken.ofSubst (ρ : Γ ⊆ʷ Δ) : Subst Γ Δ :=
+  λ _ => Term.var ∘ ρ.apply
+instance : Coe (Γ ⊆ʷ Δ) (Subst Γ Δ) := ⟨Weaken.ofSubst⟩
+
+theorem Weaken.lift_of_subst {ρ : Γ ⊆ʷ Δ} :
+  (⇑ʷρ : Γ,' T ⊆ʷ Δ,' T).ofSubst = ⇑ρ.ofSubst := by
+  funext _ x
+  cases x <;> simp [Weaken.ofSubst, Subst.lift, Term.shift]
+
+theorem Term.weaken_eq_subst {ρ : Γ ⊆ʷ Δ} : t[ρ]ʷ = t[ρ]ˢ := by
+  induction t generalizing Δ
+  case lam t ih =>
+    simp [ih]
+    congr
+    funext _ x
+    cases x
+    · rfl
+    · simp [Weaken.ofSubst, Subst.lift, Term.shift]
+  all_goals aesop
+
+def Subst.comp (σ₁ : Subst Γ Δ) (σ₂ : Subst Δ Θ) : Subst Γ Θ :=
+  λ _ x => (σ₁ x)[σ₂]ˢ
+infix:70 " ∘ₛ " => Subst.comp
+
+lemma Term.weaken_comp_subst {ρ : Γ ⊆ʷ Δ} {σ : Subst Δ Θ} :
+  t[ρ]ʷ[σ]ˢ = t[ρ ∘ₛ σ]ˢ := by
+  induction t generalizing Δ Θ
+  case lam _ ih =>
+    simp [ih]
+    congr
+    funext _ x
+    cases x
+    · rfl
+    · simp [Subst.comp, Subst.lift]
+  all_goals aesop
+
+lemma Term.subst_comp_weaken {t : Term Γ T} {σ : Subst Γ Δ} {ρ : Δ ⊆ʷ Θ} :
+  t[σ]ˢ[ρ]ʷ = t[σ ∘ₛ ρ]ˢ := by
+  induction t generalizing Δ Θ
+  case var x => simp [Term.weaken, Subst.comp, weaken_eq_subst]
+  case lam _ ih =>
+    simp [ih]
+    congr
+    funext _ x
+    cases' x with _ _ x
+    · rfl
+    · simp [Subst.comp, Subst.lift, Term.shift]
+      conv =>
+        rhs
+        rw [weaken_eq_subst]
+        arg 1
+        rw [←weaken_eq_subst]
+      simp [weaken_comp_subst]
+      congr
+      funext x
+      cases x <;> simp [Subst.comp, Weaken.ofSubst]
+  all_goals aesop
+
+theorem Term.shift_subst_lift :
+  (↑ₜt : Term (Γ,' T') T)[⇑σ]ˢ = ↑ₜ(t[σ]ˢ) := by
+  simp [Term.shift, weaken_comp_subst, subst_comp_weaken]
+  congr
+  funext x
+  simp [Subst.comp, Subst.lift, Term.shift, weaken_eq_subst]
+
+theorem Term.subst_comp {t : Term Γ T} {σ₁ : Subst Γ Δ} {σ₂ : Subst Δ Θ} :
+  t[σ₁]ˢ[σ₂]ˢ = t[σ₁ ∘ₛ σ₂]ˢ := by
+  induction t generalizing Δ Θ
+  case lam _ ih =>
+    simp [ih]
+    congr
+    funext _ x
+    cases x
+    · rfl
+    · simp [Subst.comp, Term.shift]
+      repeat conv in (⇑_ _) => simp [Subst.lift]
+      apply shift_subst_lift
+  all_goals aesop
+
+theorem Term.shift_subst_single : (↑ₜt)[↦ t']ˢ = t := by
+  simp [Term.shift, weaken_comp_subst]
+  conv => rhs; rw [←subst_id (t := t)]
+  congr
+  funext x
+  cases x <;> simp [Subst.comp, Subst.single, Subst.id]
+
+lemma substitution {t : Term (Γ,' T') T} {σ : Subst Γ Δ} :
+  t[↦ t']ˢ[σ]ˢ = t[⇑σ]ˢ[↦ (t'[σ]ˢ)]ˢ := by
+  simp [Term.subst_comp]
+  congr
+  funext _ x
+  cases x
+  · rfl
+  · simp [Subst.comp, Subst.lift, Term.shift_subst_single]
+
+lemma substitution_weaken {t : Term (Γ,' T') T} :
+  t[↦ t']ˢ[ρ]ʷ = t[⇑ʷρ]ʷ[↦ (t'[ρ]ʷ)]ˢ := by
+  simp [Term.weaken_eq_subst, Weaken.lift_of_subst]
+  apply substitution
+
+
+
+open Term in
+inductive Context (Γ : Con) (T : Ty) : Con → Ty → Type where
+| hole : Context Γ T Γ T
+| lam : Context Γ T (Δ,' T₁) T₂ → Context Γ T Δ (T₁ ⇒ T₂)
+| app₁ : Context Γ T Δ (T₁ ⇒ T₂) → Term Δ T₁ → Context Γ T Δ T₂
+| app₂ : Term Δ (T₁ ⇒ T₂) → Context Γ T Δ T₁ → Context Γ T Δ T₂
+| fix : Context Γ T Δ (T' ⇒ T') → Context Γ T Δ T'
+| ite₁ : Context Γ T Δ TBool → Term Δ T' → Term Δ T' → Context Γ T Δ T'
+| ite₂ : Term Δ TBool → Context Γ T Δ T' → Term Δ T' → Context Γ T Δ T'
+| ite₃ : Term Δ TBool → Term Δ T' → Context Γ T Δ T' → Context Γ T Δ T'
+| succ : Context Γ T Δ TNat → Context Γ T Δ TNat
+| pred : Context Γ T Δ TNat → Context Γ T Δ TNat
+| isz : Context Γ T Δ TNat → Context Γ T Δ TBool
+| pair₁ : Context Γ T Δ T₁ → Term Δ T₂ → Context Γ T Δ (T₁ * T₂)
+| pair₂ : Term Δ T₁ → Context Γ T Δ T₂ → Context Γ T Δ (T₁ * T₂)
+| fst : Context Γ T Δ (T₁ * T₂) → Context Γ T Δ T₁
+| snd : Context Γ T Δ (T₁ * T₂) → Context Γ T Δ T₂
+
+def Context.plug : Context Γ T Δ T' → Term Γ T → Term Δ T'
+| hole, t => t
+| lam C, t => λ' (C.plug t)
+| app₁ C t₂, t => C.plug t ⬝ t₂
+| app₂ t₁ C, t => t₁ ⬝ C.plug t
+| fix C, t => Term.fix (C.plug t)
+| ite₁ C t₂ t₃, t => Term.ite (C.plug t) t₂ t₃
+| ite₂ t₁ C t₃, t => Term.ite t₁ (C.plug t) t₃
+| ite₃ t₁ t₂ C, t => Term.ite t₁ t₂ (C.plug t)
+| succ C, t => Term.succ (C.plug t)
+| pred C, t => Term.pred (C.plug t)
+| isz C, t => Term.isz (C.plug t)
+| pair₁ C t₂, t => ⟪C.plug t, t₂⟫
+| pair₂ t₁ C, t => ⟪t₁, C.plug t⟫
+| fst C, t => Term.fst (C.plug t)
+| snd C, t => Term.snd (C.plug t)
+
+end PCF
